wip

crypto/bignum/Hacl.Bignum.Fmul.Spec.fst
@@ -1,5 +1,7 @@
 module Hacl.Bignum.Fmul.Spec
 
+open FStar.Mul
+
 open Hacl.Bignum.Constants
 open Hacl.Bignum.Parameters
 open Hacl.Bignum.Bigint
@@ -10,6 +12,8 @@ open Hacl.Bignum.Fproduct.Spec
 module U32 = FStar.UInt32
 
 
+#set-options "--initial_fuel 0 --max_fuel 0 --z3rlimit 5"
+
 let shift_reduce_pre (s:seqelem) : GTot Type0 = reduce_pre (shift_spec s)
 
 
@@ -17,6 +21,22 @@ val shift_reduce_spec: s:seqelem{shift_reduce_pre s} -> Tot (s':seqelem)
 let shift_reduce_spec s =
   reduce_spec (shift_spec s)
 
+#set-options "--initial_fuel 0 --max_fuel 0 --z3rlimit 100"
+
+val lemma_shift_spec_eq: s:seqelem -> Lemma
+  (Seq.append (Seq.slice (shift_spec s) 1 (len)) (Seq.slice (shift_spec s) 0 1) == s)
+let lemma_shift_spec_eq s =
+  Seq.lemma_eq_intro (Seq.append (Seq.slice (shift_spec s) 1 (len)) (Seq.slice (shift_spec s) 0 1)) (s)
+
+
+val lemma_shift_reduce_spec: s:seqelem{shift_reduce_pre s} -> Lemma
+  (seval (shift_reduce_spec s) % prime = (pow2 limb_size * seval s) % prime)
+let lemma_shift_reduce_spec s =
+  lemma_shift_spec_eq s;
+  lemma_reduce_spec (shift_spec s)
+
+
+#set-options "--initial_fuel 1 --max_fuel 1 --z3rlimit 50"
 
 let rec mul_shift_reduce_pre (output:seqelem_wide) (input:seqelem) (input2:seqelem) (ctr:nat{ctr <= len}) : GTot Type0 (decreases ctr) =
   if ctr > 0 then (
@@ -28,22 +48,138 @@ let rec mul_shift_reduce_pre (output:seqelem_wide) (input:seqelem) (input2:seqel
           else true
 
 
-val mul_shift_reduce_spec:
+#set-options "--z3rlimit 10 --initial_fuel 1 --max_fuel 1"
+
+assume val lemma_mod_mul_distr: a:nat -> b:nat -> p:pos -> Lemma ((a+b)%p = ((a%p) + b) % p)
+assume val lemma_mod_mul_comm: a:nat -> b:nat -> p:pos -> Lemma ((a*b)%p = ((a%p)*b)%p)
+
+
+(* val mul_shift_reduce_spec_step_1: o1:nat -> o2:nat -> i0:nat -> i1:nat -> i2:nat -> x:nat -> ctr:nat -> Lemma *)
+(*   (requires (o2 = o1 + i1 * x /\ i1 % p = pow2 ((len - ctr) * limb_size) * i0 % p)) *)
+(*   (ensures (o2 % p = (pow2 ((len-ctr)*limb_size) * i0 * x))) *)
+
+
+(* val mul_shift_reduce_spec_step: *)
+(*   output:seqelem_wide -> *)
+(*   input_init:seqelem -> *)
+(*   input:seqelem -> *)
+(*   input2:seqelem -> *)
+(*   ctr:pos{ctr <= len /\ mul_shift_reduce_pre output input input2 ctr *)
+(*     /\ (ctr > 0 ==> seval input % prime = pow2 ((len - ctr) * limb_size) * seval input_init % prime) *)
+(*     /\ seval_wide output % prime = (seval input_init * seval_ input2 (len - ctr)) % prime} -> *)
+(*   Tot (s:seqelem_wide{((ctr = 1) ==> seval_wide s % prime = (seval input * seval input2) % prime) *)
+(*     /\ (ctr <> 1 ==> seval_wide s % prime = (seval input_init * seval_ input2 (len-ctr+1)) % prime)}) *)
+(* let mul_shift_reduce_spec_step output input_init input input2 ctr = *)
+(*   let i = ctr - 1 in *)
+(*   let j = len - i - 1 in *)
+(*   let input2j = Seq.index input2 j in *)
+(*   let output' = sum_scalar_multiplication_spec output input input2j len in *)
+(*   lemma_sum_scalar_multiplication_ output input input2j len; *)
+(*   cut (seval_wide output' = seval_wide output + (seval input * v input2j)); *)
+(*   Math.Lemmas.nat_times_nat_is_nat (seval input) (v input2j); *)
+(*   let input'  = if ctr > 1 then shift_reduce_spec input else input in *)
+(*   if ctr = 1 then ( *)
+(*     (\* admit(); *\) *)
+(*     (\* let o1 = seval_wide output in *\) *)
+(*     (\* let o2 = seval_wide output' in *\) *)
+(*     (\* let p = prime in *\) *)
+(*     (\* let i0 = seval input_init in *\) *)
+(*     (\* let i1 = seval input in *\) *)
+(*     (\* lemma_mod_mul_distr (seval_wide output) (seval input * v input2j) prime; *\) *)
+(*     (\* cut (seval_wide output' % prime = ((seval input_init * seval_ input2 (len-1)) % prime *\) *)
+(*     (\*                                   + seval input * v input2j) % prime); *\) *)
+(*     (\* lemma_mod_mul_distr (seval input_init * seval_ input2 (len-1)) (seval input * v input2j) prime; *\) *)
+(*     (\* cut (seval_wide output' % prime = (seval input_init * seval_ input2 (len-1) *\) *)
+(*     (\*                                   + seval input * v input2j) % prime); *\) *)
+(*     (\* lemma_mod_mul_distr (seval input * v input2j) (seval input_init * seval_ input2 (len-1)) prime; *\) *)
+(*     (\* lemma_mod_mul_distr (seval input_init * v input2j) (seval input_init * seval_ input2 (len-1)) prime; *\) *)
+(*     (\* cut (seval_wide output' % prime = *\) *)
+(*     (\*   (seval input_init * seval_ input2 (len-1) + seval input_init * pow2 (limb_size * (len-1)) * v input2j) % prime); *\) *)
+(*     (\* () *\) *)
+(*     assume (seval_wide output' % prime = (seval input_init * seval input2) % prime); *)
+(*   ) else ( *)
+(*     (\* cut (seval_wide output' = seval_wide output + (seval input * v input2j)); *\) *)
+(*     (\* cut (seval input' % prime = seval input + (pow2 limb_size * seval input) % prime); *\) *)
+(*     admit() *)
+(*   ); *)
+
+#set-options "--z3rlimit 10 --initial_fuel 0 --max_fuel 0"
+
+val mul_shift_reduce_spec_:
   output:seqelem_wide ->
-  input:seqelem -> input2:seqelem ->
-  ctr:nat{ctr <= len /\ mul_shift_reduce_pre output input input2 ctr} ->
-  Tot seqelem_wide
+  input_init:seqelem ->
+  input:seqelem ->
+  input2:seqelem ->
+  ctr:nat{ctr <= len /\ mul_shift_reduce_pre output input input2 ctr
+    /\ seval_wide output % prime = (seval input * seval_ input2 (len - ctr)) % prime
+    /\ (ctr > 0 ==> seval input % prime = (pow2 ((len - ctr) * limb_size) * seval input_init) % prime)
+    } ->
+  Tot (s:seqelem_wide{seval_wide s % prime = (seval input * seval input2) % prime})
   (decreases ctr)
-let rec mul_shift_reduce_spec output input input2 ctr =
+
+#set-options "--z3rlimit 50 --initial_fuel 1 --max_fuel 1"
+
+let rec mul_shift_reduce_spec_ output input_init input input2 ctr =
   if ctr = 0 then output
   else (
     let i = ctr - 1 in
     let j = len - i - 1 in
     let input2j = Seq.index input2 j in
     let output' = sum_scalar_multiplication_spec output input input2j len in
+    lemma_sum_scalar_multiplication_ output input input2j len;
+    cut (seval_wide output' = seval_wide output + (seval input * v input2j));
     let input'  = if ctr > 1 then shift_reduce_spec input else input in
-    mul_shift_reduce_spec output' input' input2 i
+    if ctr = 1 then (
+      lemma_mod_mul_distr (seval_wide output) (seval input * v input2j) prime;
+      cut (seval_wide output' % prime = ((seval input * seval_ input2 (len-1)) % prime + seval input * v input2j) % prime);
+      admit() (* TODO *)
+    );
+    admit();  (* TODO *)
+    mul_shift_reduce_spec_ output' input_init input' input2 i
   )
+
+
+val lemma_seval_wide_null: a:seqelem_wide -> ctr:nat{ctr <= len} -> Lemma
+  (requires (a == Seq.create len wide_zero))
+  (ensures (seval_wide_ a ctr = 0))
+let rec lemma_seval_wide_null a ctr =
+  if ctr = 0 then () else lemma_seval_wide_null a (ctr-1)
+
+
+val mul_shift_reduce_spec:
+  input:seqelem -> input2:seqelem{mul_shift_reduce_pre (Seq.create len wide_zero) input input2 len} ->
+  Tot (s:seqelem_wide{seval_wide s % prime = (seval input * seval input2) % prime})
+let rec mul_shift_reduce_spec input input2 =
+  lemma_seval_wide_null (Seq.create len wide_zero) len;
+  assert_norm (pow2 0 = 1);
+  mul_shift_reduce_spec_ (Seq.create len wide_zero) input input input2 len
+
+
+#set-options "--z3rlimit 5 --initial_fuel 2 --max_fuel 2"
+
+(* val lemma_mul_shift_reduce_spec_: *)
+(*   output:seqelem_wide -> *)
+(*   input:seqelem -> input2:seqelem -> *)
+(*   ctr:nat{ctr <= len /\ mul_shift_reduce_pre output input input2 ctr} -> *)
+(*   Lemma *)
+(*     ((seval_wide (mul_shift_reduce_spec_ output input input2 ctr)) % prime *)
+(*     = (seval input * seval_ input2 (len - ctr)) % prime) *)
+(* let rec lemma_mul_shift_reduce_spec_ input input2 ctr = *)
+(*   if ctr = 0 then ( *)
+(*     lemma_seval_wide_null (mul_shift_reduce_spec input input2 ctr) len *)
+(*   ) else ( *)
+(*     let zeros = Seq.create len wide_zero in *)
+(*     let s = sum_scalar_multiplication_spec zeros input (Seq.index input2 (len-ctr-1)) in *)
+(*     let input' = if ctr = 1 then input else shift_reduce_spec input in *)
+(*     lemma_mul_shift_reduce_spec_ input' input2 (ctr-1); *)
+(*     admit(); *)
+(*     if ctr = 1 then ( *)
+(*       (\* lemma_seval_wide_null (mul_shift_reduce_spec input input2 0) len; *\) *)
+(*       (\* assert(seval_wide (mul_shift_reduce_spec input input2 (ctr-1)) % prime = 0); *\) *)
+(*       admit() *)
+(*     ) *)
+(*     else admit() *)
+(*   ) *)
 
 
 let fmul_pre (input:seqelem) (input2:seqelem) : GTot Type0 =
