crypto/bignum/Hacl.Bignum.Fscalar.Spec.fst
@@ -11,7 +11,7 @@ module U32 = FStar.UInt32
 
 #set-options "--initial_fuel 1 --max_fuel 1 --z3rlimit 20"
 
-val fscalar_spec:
+val fscalar_spec_:
   output:seqelem_wide -> input:seqelem -> s:limb -> ctr:nat{ctr <= len} ->
   Tot (s':seqelem_wide{
     (forall (i:nat). {:pattern (w (Seq.index s' i))} i < ctr ==>
@@ -20,34 +20,49 @@ val fscalar_spec:
               Seq.index s' i == Seq.index output i)
        })
   (decreases ctr)
-let rec fscalar_spec output input s ctr =
+let rec fscalar_spec_ output input s ctr =
   if ctr = 0 then output
   else (
     let i = ctr - 1 in
     let inputi = Seq.index input i in
     let open Hacl.Bignum.Wide in
     let output' = Seq.upd output i (inputi *^ s) in
-    fscalar_spec output' input s i
+    fscalar_spec_ output' input s i
   )
 
-#set-options "--initial_fuel 1 --max_fuel 1 --z3rlimit 50"
+
+val fscalar_spec:
+  input:seqelem -> s:limb ->
+  Tot (s':seqelem_wide{(forall (i:nat). {:pattern (w (Seq.index s' i))} i < len ==>
+                          w (Seq.index s' i) = v (Seq.index input i) * v s) })
+let fscalar_spec input s = fscalar_spec_ (Seq.create len wide_zero) input s len
+
+
+#set-options "--initial_fuel 1 --max_fuel 1 --z3rlimit 100"
 
 val lemma_fscalar_eval_:  a:seqelem_wide -> b:seqelem -> s:limb ->
   ctr:nat{ctr <= len} ->
-  Lemma (seval_wide_ (fscalar_spec a b s len) ctr = seval_ b ctr * v s)
+  Lemma (seval_wide_ (fscalar_spec_ a b s len) ctr = seval_ b ctr * v s)
 let rec lemma_fscalar_eval_ a b s ctr =
   if ctr = 0 then ()
   else (
     lemma_fscalar_eval_ a b s (ctr-1);
-    cut (seval_wide_ (fscalar_spec a b s len) (ctr-1) = seval_ b (ctr-1) * v s);
-    cut (w (Seq.index (fscalar_spec a b s len) (ctr-1)) = v (Seq.index b (ctr-1)) * v s);
-    let x = fscalar_spec a b s len in
+    cut (seval_wide_ (fscalar_spec_ a b s len) (ctr-1) = seval_ b (ctr-1) * v s);
+    cut (w (Seq.index (fscalar_spec_ a b s len) (ctr-1)) = v (Seq.index b (ctr-1)) * v s);
+    let x = fscalar_spec_ a b s len in
     cut (seval_wide_ x ctr = pow2 (limb_size * (ctr-1)) * (w (Seq.index x (ctr-1))) + seval_wide_ x (ctr-1));
     cut (seval_ b ctr = pow2 (limb_size * (ctr-1)) * (v (Seq.index b (ctr-1))) + seval_ b (ctr-1));
     Math.Lemmas.distributivity_add_left (seval_ b (ctr-1)) (pow2 (limb_size * (ctr-1)) * (v (Seq.index b (ctr-1)))) (v s)
   )
 
 
-val lemma_fscalar_eval:  a:seqelem_wide -> b:seqelem -> s:limb ->
-  Lemma (seval_wide_ (fscalar_spec a b s len) len = seval_ b len * v s)
-let rec lemma_fscalar_eval a b s = lemma_fscalar_eval_ a b s len
+val lemma_fscalar_eval_0: a:seqelem_wide -> b:seqelem -> s:limb -> Lemma
+  (fscalar_spec b s == fscalar_spec_ a b s len)
+let lemma_fscalar_eval_0 a b s =
+  let s0 = fscalar_spec b s in
+  let s1 = fscalar_spec_ a b s len in
+  assert(forall (i:nat). i < len ==> w (Seq.index s0 i) == w (Seq.index s1 i));
+  Seq.lemma_eq_intro (fscalar_spec b s) (fscalar_spec_ a b s len)
+
+val lemma_fscalar_eval: b:seqelem -> s:limb -> Lemma (seval_wide (fscalar_spec b s) = seval b * v s)
+let rec lemma_fscalar_eval b s = lemma_fscalar_eval_ (Seq.create len wide_zero) b s len
