crypto/bignum/Hacl.Bignum.fst
@@ -42,6 +42,12 @@ let fsum a b =
   Hacl.Bignum.Fsum.Spec.lemma_fsum_eval (as_seq h0 a) (as_seq h0 b)
 
 
+assume val lemma_diff: a:int -> b:int -> p:pos ->
+  Lemma ( (a - b) % p = ((a%p) - b) % p /\ (a - b) % p = (a - (b % p)) % p)
+
+
+#set-options "--z3rlimit 20"
+
 val fdifference:
   a:felem ->
   b:felem{disjoint a b} ->
@@ -54,7 +60,6 @@ val fdifference:
 let fdifference a b =
   let hinit = ST.get() in
   push_frame();
-  let h0 = ST.get() in
   let tmp = create limb_zero clen in
   blit b 0ul tmp 0ul clen;
   let h = ST.get() in
@@ -63,14 +68,14 @@ let fdifference a b =
   FStar.Seq.lemma_eq_intro (as_seq h b) (as_seq h tmp);
   add_zero tmp;
   let h' = ST.get() in
-  cut (eval h' tmp % prime = eval hinit b % prime); admit()
+  cut (eval h' tmp % prime = eval hinit b % prime);
   fdifference_ a tmp clen;
   let h1 = ST.get() in
   Hacl.Bignum.Fdifference.Spec.lemma_fdifference_eval (as_seq hinit a) (as_seq h' tmp);
-  cut (eval h1 a = eval h' tmp - eval hinit a); admit()
-  pop_frame();
-  let hfin = ST.get() in
-  assume (eval hfin a % prime = (eval hinit b - eval hinit a) % prime)
+  lemma_diff (eval h' tmp) (eval hinit a) prime;
+  lemma_diff (eval hinit b) (eval hinit a) prime;
+  pop_frame()
+
 
 open Hacl.Bignum.Fscalar.Spec
 open Hacl.Bignum.Fproduct.Spec
@@ -81,24 +86,26 @@ val fscalar:
   s:limb ->
   Stack unit
     (requires (fun h -> live h b /\ live h a
-      /\ carry_wide_pre (fscalar_spec (Seq.create len wide_zero) (as_seq h b) s len) 0
-      /\ carry_top_wide_pre (carry_wide_spec (fscalar_spec (Seq.create len wide_zero) (as_seq h b) s len) 0)
-      /\ copy_from_wide_pre (carry_top_wide_spec (carry_wide_spec (fscalar_spec (Seq.create len wide_zero) (as_seq h b) s len) 0)) ))
+      /\ carry_wide_pre (fscalar_spec (as_seq h b) s) 0
+      /\ carry_top_wide_pre (carry_wide_spec (fscalar_spec (as_seq h b) s) 0)
+      /\ copy_from_wide_pre (carry_top_wide_spec (carry_wide_spec (fscalar_spec (as_seq h b) s) 0)) ))
     (ensures (fun h0 _ h1 -> live h0 a /\ live h0 b /\ modifies_1 a h0 h1 /\ live h1 a
-      /\ eval h1 a = eval h0 b * v s))
+      /\ eval h1 a % prime = (eval h0 b * v s) % prime))
 let fscalar output b s =
   let hinit = ST.get() in
   push_frame();
-  let h0 = ST.get() in
   let tmp = create wide_zero clen in
   fscalar tmp b s;
+  lemma_fscalar_eval (as_seq hinit b) s;
   carry_wide_ tmp 0ul;
+  let h' = ST.get() in
+  cut (eval_wide h' tmp = eval hinit b * v s);
   carry_top_wide tmp;
+  let h'' = ST.get() in
+  lemma_carry_top_wide_spec (as_seq h' tmp);
   copy_from_wide_ output tmp clen;
-  let h1 = ST.get() in
-  pop_frame();
-  let hfin = ST.get() in
-  assume (eval hfin output = eval hinit b * v s)
+  lemma_copy_from_wide (as_seq h'' tmp);
+  pop_frame()
 
 
 val fmul:
@@ -108,7 +115,7 @@ val fmul:
   Stack unit
     (requires (fun h -> live h output /\ live h a /\ live h b
       /\ fmul_pre (as_seq h a) (as_seq h b)))
-    (ensures (fun h0 _ h1 -> live h0 output /\ live h0 output /\ live h0 a /\ live h0 b 
+    (ensures (fun h0 _ h1 -> live h0 output /\ live h0 output /\ live h0 a /\ live h0 b
       /\ modifies_1 output h0 h1 /\ live h1 output
       /\ eval h1 output % prime = (eval h0 a * eval h0 b) % prime
       ))
