crypto/bignum/Hacl.Bignum.Fmul.Lemmas.fsti
@@ -13,7 +13,7 @@ module U32 = FStar.UInt32
 val lemma_mul_to_red: input:seqelem -> input2:seqelem -> Lemma
   (requires (fmul_pre input input2))
   (ensures  (fmul_pre input input2
-    /\ carry_wide_pre (mul_shift_reduce_spec (Seq.create len wide_zero) input input2 len) 0
-    /\ carry_top_wide_pre (carry_wide_spec (mul_shift_reduce_spec (Seq.create len wide_zero) input input2 len) 0)
-    /\ copy_from_wide_pre (carry_top_wide_spec (carry_wide_spec (mul_shift_reduce_spec (Seq.create len wide_zero) input input2 len) 0))
-    /\ carry_0_to_1_pre (copy_from_wide_spec (carry_top_wide_spec (carry_wide_spec (mul_shift_reduce_spec (Seq.create len wide_zero) input input2 len) 0)))))
+    /\ carry_wide_pre (mul_shift_reduce_spec input input2) 0
+    /\ carry_top_wide_pre (carry_wide_spec (mul_shift_reduce_spec input input2) 0)
+    /\ copy_from_wide_pre (carry_top_wide_spec (carry_wide_spec (mul_shift_reduce_spec input input2) 0))
+    /\ carry_0_to_1_pre (copy_from_wide_spec (carry_top_wide_spec (carry_wide_spec (mul_shift_reduce_spec input input2) 0)))))
